Add uncleaned updates (will be cleaned tomorrow)

complete-theory/compositionalityScript.sml
@@ -1,6 +1,10 @@
-
 open HolKernel boolLib bossLib Parse bagTheory listTheory
 val _ = new_theory "compositionality";
+
+Datatype:
+  C         = Q α | Composition C C ;
+  S         = P (α set) | Conjunction S S | Contract S S | Parallell S S
+End
 
 val _ = add_rule
   {term_name = "Contract", fixity = Closefix,
@@ -16,7 +20,7 @@ val _ = add_rule {block_style = (AroundEachPhrase, (PP.INCONSISTENT, 2)),
                   fixity = Infix(NONASSOC, 450),
                   paren_style = OnlyIfNecessary,
                   pp_elements = [TOK "◁"],
-                  term_name = "Impl"}
+                  term_name = "Implements"}
 
 val _ = add_rule {block_style = (AroundEachPhrase, (PP.INCONSISTENT, 2)),
                   fixity = Infix(NONASSOC, 550),
@@ -28,7 +32,7 @@ val _ = add_rule {block_style = (AroundEachPhrase, (PP.INCONSISTENT, 2)),
                   fixity = Infix(NONASSOC, 580),
                   paren_style = OnlyIfNecessary,
                   pp_elements = [TOK "⊓"],
-                  term_name = "And"}
+                  term_name = "Conjunction"}
 
 val _ = add_rule {block_style = (AroundEachPhrase, (PP.CONSISTENT, 0)),
                   fixity = Infixl 581,
@@ -36,39 +40,49 @@ val _ = add_rule {block_style = (AroundEachPhrase, (PP.CONSISTENT, 0)),
                   pp_elements = [TOK "ₓ"],
                   term_name = "Composition"}
 
-
-Datatype:
-  Term = Impl C S | Assertional S | Refines S S ;
-  C    = Q α | Composition C C ;
-  S    = P (α set) | And S S | Contract S S | Parallell S S
-End
-
 Definition C_M:
-    C_M (Q α)     = {α}
+    C_M (Q α)     = α
   ∧ C_M (c1 ₓ c2) = (C_M c1) ∩ (C_M c2)
 End
 
 Definition S_M:
-    (S_M (P α)             = {α})
+    (S_M (P α)             = α)
   ∧ (S_M (s1 ⊓ s2)         = (S_M s1) ∩ (S_M s2))
-  ∧ (S_M (s1, s2)          = {b | ∀b'. C_M b' ∈ S_M s1 ⇒ C_M b' ∩ b ∈ S_M s2})
+  ∧ (S_M (s1, s2)          = {b | ∀b'. b' ∈ S_M s1 ⇒ b' ∩ b ∈ S_M s2})
   ∧ (S_M (Parallell s1 s2) = {a ∩ b | a ∈ (S_M s1) ∧ b ∈ (S_M s2)})
 End
 
-Definition T_M:
-    (T_M (c ◁ s)      ⇔ C_M c ∈ S_M s)
-  ∧ (T_M (s1 ⊑ s2)     ⇔ S_M s1 ⊆ S_M s2)
+Definition Implements:
+    Implements c s ⇔ C_M c ∈ S_M s
 End
 
-Theorem IMPL_AX_THM:
-  ∀c s. T_M (c ◁ s) ⇔ C_M c ∈ S_M s 
+Definition Refines:
+    Refines s1 s2 ⇔ S_M s1 ⊆ S_M s2
+End
+
+Theorem IMPLEMENTS_AX_THM:
+  ∀c s. c ◁ s ⇔ C_M c ∈ S_M s 
 Proof
   EVAL_TAC >>
   rw[]
 QED
 
+Theorem COMP_EX_THM:
+  ∀s. C_M (Q s) = s
+Proof
+  EVAL_TAC >>
+  rw[]
+QED
+
+Theorem COMP_IMPL_EX_THM:
+  ∀s. ∃s'. C_M s' = s
+Proof
+  ASSUME_TAC COMP_EX_THM >>
+  metis_tac[]
+QED
+
 Theorem COMP_ASSOC_THM:
-  ∀c1 c2 c3 s. T_M (c1 ₓ c2 ₓ c3 ◁ s) ⇔ T_M (c1 ₓ (c2 ₓ c3) ◁ s)
+  ∀c1 c2 c3 s. c1 ₓ c2 ₓ c3 ◁ s ⇔ c1 ₓ (c2 ₓ c3) ◁ s
 Proof
   EVAL_TAC >>
   rw[] >>
@@ -76,7 +90,7 @@ Proof
 QED
 
 Theorem COMP_COMM_THM:
-  ∀c1 c2 s. T_M (c1 ₓ c2 ◁ s) ⇔ T_M (c2 ₓ c1 ◁ s)
+  ∀c1 c2 s. c1 ₓ c2 ◁ s ⇔ c2 ₓ c1 ◁ s
 Proof
   EVAL_TAC >>
   rw[] >>
@@ -84,64 +98,178 @@ Proof
 QED
 
 Theorem ELEM_IN_AND_THM:
-  ∀e s1 s2. e ∈ S_M s1 ∧ e ∈ S_M s2 ⇒ e ∈ S_M (s1 ⊓ s2)
+  ∀e s1 s2. e ∈ S_M s1 ∧ e ∈ S_M s2 ⇔ e ∈ S_M (s1 ⊓ s2)
 Proof
   EVAL_TAC >>
   rw[]
 QED
 
 Theorem AND_THM:
-  ∀c s1 s2. T_M (c ◁ s1) ∧ T_M (c ◁ s2) ⇒ T_M (c ◁ s1 ⊓ s2)
+  ∀c s1 s2. c ◁ s1 ∧ c ◁ s2 ⇔ c ◁ s1 ⊓ s2
 Proof
-  rw[] >>
-  metis_tac[IMPL_AX_THM, ELEM_IN_AND_THM]
+  EVAL_TAC >>
+  rw[]
 QED
 
 Theorem AND_ELIM_1_THM:
-  ∀c s1 s2. T_M (c ◁ s1 ⊓ s2) ⇒ T_M (c ◁ s2)
+  ∀c s1 s2. c ◁ s1 ⊓ s2 ⇒ c ◁ s2
 Proof
   EVAL_TAC >>
   rw[]
 QED
 
 Theorem AND_ELIM_2_THM:
-  ∀c s1 s2. T_M (c ◁ s1 ⊓ s2) ⇒ T_M (c ◁ s1)
+  ∀c s1 s2. c ◁ s1 ⊓ s2 ⇒ c ◁ s1
 Proof
   EVAL_TAC >>
   rw[]
 QED
 
 Theorem REFINEMENT_THM:
-  ∀c s1 s2. T_M (c ◁ s1) ∧ T_M (s1 ⊑ s2) ⇒ T_M (c ◁ s2)
+  ∀c s1 s2. c ◁ s1 ∧ s1 ⊑ s2 ⇒ c ◁ s2
 Proof
   EVAL_TAC >>
   metis_tac[pred_setTheory.SUBSET_DEF, pred_setTheory.SUBSET_TRANS]
 QED
 
 Theorem CONTRACT_ELIM_THM:
-  ∀c1 c2 s1 s2. T_M (c1 ◁ s1) ∧ T_M(c2 ◁ (s1, s2)) ⇒ T_M (c1 ₓ c2 ◁ s2)
+  ∀c1 c2 s1 s2. c1 ◁ s1 ∧ c2 ◁ (s1, s2) ⇒ c1 ₓ c2 ◁ s2
 Proof
   EVAL_TAC >>
   rw[]
 QED
 
-Theorem SPEC_CONTRACT_INTRO_THM:
-  ∀c2 s1 s2. (∀q0. T_M (q0 ◁ s1) ⇒ T_M (q0 ₓ c2 ◁ s2)) ⇒ T_M (c2 ◁ (s1,s2))
+Theorem CONTRACT_INTRO_THM:
+  ∀q0 c s1 s2. (∀q0. (q0 ◁ s1) ⇒ q0 ₓ c ◁ s2) ⇒ c ◁ (s1,s2)
 Proof
   EVAL_TAC >>
-  rw[]
+  rw[] >>
+  metis_tac[COMP_IMPL_EX_THM]
+QED
+
+val Assertional_AX =
+ new_axiom("Assertional_AX", “∀c1 c2 s. c1 ◁ s ∧ Assertional(s) ⇒ c1 ₓ c2 ◁ s”);
+
+val comp_rules = [CONTRACT_ELIM_THM,
+                  CONTRACT_INTRO_THM,
+                  REFINEMENT_THM,
+                  COMP_ASSOC_THM,
+                  COMP_COMM_THM,
+                  Assertional_AX];
+
+Theorem PAPER_EXAMPLE:
+  Assertional(a) ∧
+  a ⊑ a1 ∧
+  a ⊓ g1 ⊑ a2 ∧
+  g2 ⊑ g ∧
+  c1 ◁ (a1, g1) ∧
+  c2 ◁ (a2, g2)
+  ⇒
+  c1 ₓ c2 ◁ (a, g)
+Proof
+  rw[] >>
+  metis_tac comp_rules
+QED
+
+val comp_rules = [CONTRACT_ELIM_THM,
+                  CONTRACT_INTRO_THM,
+                  REFINEMENT_THM,
+                  COMP_ASSOC_THM,
+                  COMP_COMM_THM];
+
+Theorem PAPER_EXAMPLE:
+  Refines a a1 ∧
+  Refines g1 a2 ∧
+  Refines g2 g ∧
+          c1 ◁ (a1, g1) ∧ c2 ◁ (a2, g2) ⇒ c1 ₓ c2 ◁ (a, g)
+Proof
+  rw[] >>
+  sg ‘∀q0. (q0 ◁ a) ⇒ q0 ₓ c1 ₓ c2 ◁ g’ >>
+  rw[] >>
+  >- ‘q0 ◁ a1’ by metis_tac[REFINEMENT_THM] >>
+     ‘q0 ₓ c1 ◁ g1’ by metis_tac[CONTRACT_ELIM_THM] >>
+     ‘q0 ₓ c1 ◁ a2’ by metis_tac[REFINEMENT_THM] >>
+     ‘(q0 ₓ c1) ₓ c2 ◁ g2’ by metis_tac[CONTRACT_ELIM_THM] >>
+     ‘(q0 ₓ c1) ₓ c2 ◁ g’ by metis_tac[REFINEMENT_THM] >>
+     metis_tac[CONTRACT_INTRO_THM, COMP_COMM_THM, COMP_ASSOC_THM]
+  metis_tac comp_rules
+QED
+
+
+(*
+https://github.com/HOL-Theorem-Prover/HOL/blob/develop/examples/logic/propositional_logic/IntuitionisticProofScript.sml
+*)
+
+(* todo: or intro, or elim
+*)
+Inductive G:
+    (∀f. G {f} f) (* Base case *)
+  ∧ (∀f1 f2 Γ1 Γ2. G Γ1 f1 ∧ G Γ2 f2
+         ⇒ G (Γ1 UNION Γ2) (f1 ∧ f2)) (* And Intro *)
+  ∧ (∀f1 f2 Γ. G Γ (f1 ∧ f2)
+         ⇒ G Γ f1) (* And elim left *)
+  ∧ (∀f1 f2 Γ. G Γ (f1 ∧ f2)
+         ⇒ G Γ f2) (* And elim right *)
+  ∧ (∀f1 f2 Γ. G (f1 INSERT Γ) f2
+         ⇒ G Γ (f1 ⇒ f2)) (* Imp intro *)
+  ∧ (∀f1 f2 Γ1 Γ2. G Γ2 (f1 ⇒ f2) ∧ G Γ1 f1
+         ⇒ G (Γ1 UNION Γ2) f2) (* Imp Elim *)
+End
+
+val [G_AX, G_AND_IN, G_AND_EL_R, G_AND_EL_L, G_IMP_IN, G_IMP_EL] = CONJUNCTS G_rules;
+
+Theorem G_lw:
+  ∀Γ f1. G Γ f1 ⇒ ∀f2. G (f2 INSERT Γ) f1
+Proof
+  rw[] >>
+  ‘G {f2} f2’ by metis_tac[G_AX] >>
+  ‘G ({f2} ∪ Γ) (f2 ∧ f1)’ by metis_tac[G_AND_IN] >>
+  ‘G ({f2} ∪ Γ) f1’ by metis_tac[G_AND_EL_L] >>
+  metis_tac[INSERT_SING_UNION]
+QED
+
+Theorem G_ALL:
+Proof
+QED
+
+Theorem G_AND_THM:
+  ∀c s1 s2 Γ. G Γ (c ◁ s1) ∧ G Γ (c ◁ s2) ⇒ G Γ (c ◁ s1 ⊓ s2)
+Proof
+  EVAL_TAC >>
+  rw[] >>
+  metis_tac[UNION_IDEMPOT, G_AND_IN]
+QED
+
+Theorem G_AND_EL_L_THM:
+  ∀c s1 s2 Γ. G Γ (c ◁ s1 ⊓ s2) ⇒ G Γ (c ◁ s2)
+Proof
+  EVAL_TAC >>
+  rw[] >>
+  metis_tac[G_AND_EL_L]
+QED
+
+Theorem G_AND_EL_R_THM:
+  ∀c s1 s2 Γ. G Γ (c ◁ s1 ⊓ s2) ⇒ G Γ (c ◁ s1)
+Proof
+  EVAL_TAC >>
+  rw[] >>
+  metis_tac[G_AND_EL_R]
 QED
 
 Inductive G:
-    (∀(t:α Term) Γ. (t <: Γ) ⇒ G Γ t) (* ax *)
-  ∧ (∀t1 t2 Γ. G Γ t1 ∧ (T_M t1 ⇒ T_M t2) ⇒ G Γ t2) (* lower-level-imp *)
-  ∧ (∀t1 t2 t3 Γ. G Γ t1 ∧ G Γ t2 ∧ (T_M t1 ∧ T_M t2 ⇒ T_M t3) ⇒ G Γ t3) (* lower-level-imp *)
-  ∧ (∀q0 c s1 s2 Γ. G (BAG_INSERT (q0 ◁ s1) Γ) ((q0 ₓ c) ◁ s2) ⇒ G Γ (c ◁ (s1, s2))) (* contract *)
-  ∧ (∀c1 c2 s Γ. G Γ (c1 ◁ s) ∧ BAG_IN (Assertional s) Γ ⇒ G Γ (c1 ₓ c2 ◁ s)) 
-  ∧ (∀t1 t2 Γ . G Γ t1 ⇒ G (BAG_INSERT t2 Γ) t1) (* closure *)
+    (∀t Γ. t ⇒ G Γ t) (* ax *)
+  ∧ (∀t0 t1 Γ. G (BAG_INSERT t0 Γ) t1 ⇒ G Γ (t0 ⇒ t1)) (* Right Impl *)
 End
 
-val [G_AX, G_LOWER_IMP, G_LOWER_IMP2, G_CONTRACT_AX, G_ASSERTION, G_CLOSURE] = CONJUNCTS G_rules;
+val [G_AX, G_RIGHT_IMP] = CONJUNCTS G_rules;
+
+Theorem G_CONTRACT_INTRO:
+  (∀c s1 s2 Γ. (G (BAG_INSERT (q0 ◁ s1) Γ) ((q0 ₓ c) ◁ s2)) ⇒ G Γ (c ◁ (s1, s2)))
+Proof
+  EVAL_TAC
+  rw[]
+  ‘∀q0. G Γ (C_M q0 ∈ S_M s1 ⇒ C_M q0 ∩ C_M c ∈ S_M s2)’ by metis_tac[G_RIGHT_IMP]
+QED
 
 Theorem G_REFINEMENT_THM:
   ∀c s1 s2 Γ. G Γ (c ◁ s1) ∧ (BAG_IN (s1 ⊑ s2) Γ) ⇒ G Γ (c ◁ s2)
@@ -171,16 +299,14 @@ Proof
 QED
 *)
 
-val comp_rules = [ELEM_IN_AND_THM,
-                  AND_THM,
+val comp_rules = [AND_THM,
                   AND_ELIM_1_THM,
                   AND_ELIM_2_THM,
                   CONTRACT_ELIM_THM,
-                  SPEC_CONTRACT_INTRO_THM,
+                  CONTRACT_INTRO_THM,
                   REFINEMENT_THM,
                   G_AX,
                   G_LOWER_IMP,
-                  G_LOWER_IMP2,
                   G_CONTRACT_AX,
                   G_ASSERTION,
                   G_REFINEMENT_THM,
@@ -190,18 +316,28 @@ val comp_rules = [ELEM_IN_AND_THM,
                   COMP_ASSOC_THM,
                   COMP_COMM_THM];
 (*
+
 Context menu
 
 Pallet
-*)
 
-Definition COMPOSITIONALITY_TAC:
-  COMPOSITIONALITY_TAC = metis_tac comp_rules
-End
+---
+
+Report writing!
+
+Dilian decomposition.
+
+Ethical aspects?
+
+Send dilian skeleton.
+
+---
+
+*)
 
 Theorem PAPER_EXAMPLE:
   let
-    Γ = {|Assertional a; a ⊑ a1; (a ⊓ g1) ⊑ a2; g2 ⊑ g|}
+    Γ = {|Assertional(a); a ⊑ a1; a ⊓ g1 ⊑ a2; g2 ⊑ g|}
   in
     G Γ (c1 ◁ (a1, g1)) ∧ G Γ (c2 ◁ (a2, g2)) ⇒ G Γ (c1 ₓ c2 ◁ (a, g))
 Proof
@@ -210,13 +346,18 @@ Proof
 QED
 
 Theorem FUEL_LEVEL_DISPLAY_CONTROLLER:
-    Γ = {|g_I ⊑ a_A;
-          g_ADC ⊑ a_I; g_A ⊑ a_DAC;
-          g_T ⊑ a_ADC; g_DAC ⊑ a_D;|}
-    ∧ G Γ (c_I ◁ (a_I, g_I)) ∧ G Γ (c_A ◁ (a_A, g_A)) (* Program components *)
-    ∧ G Γ (c_ADC ◁ (a_ADC, g_ADC)) ∧ G Γ (c_DAC ◁ (a_DAC, g_DAC)) (* Controller components *)
-    ∧ G Γ (c_T ◁ (a_T, g_T)) ∧ G Γ (c_D ◁ (a_D, g_D)) (* Additional system components *)
+  let
+    Γ = {|g_I ⊑ a_A; g_ADC ⊑ a_I; g_A ⊑ a_DAC; g_T ⊑ a_ADC; g_DAC ⊑ a_D;|}
+  in
+      G Γ (c_I ◁ (a_I, g_I))       (* Interface *)
+    ∧ G Γ (c_A ◁ (a_A, g_A))       (* Applet *)
+    ∧ G Γ (c_ADC ◁ (a_ADC, g_ADC)) (* ADC *)
+    ∧ G Γ (c_DAC ◁ (a_DAC, g_DAC)) (* DAC *)
+    ∧ G Γ (c_T ◁ (a_T, g_T))       (* Tank *)
+    ∧ G Γ (c_D ◁ (a_D, g_D))       (* Display *)
+
   ⇒ G Γ ((c_T ₓ c_ADC ₓ c_I ₓ c_A ₓ c_DAC ₓ c_D) ◁ (a_T, g_D))
+
 Proof
   rw[] >>
   metis_tac comp_rules
